Prefix(:=<https://w3id.org/pmd/ao/tto/>)
Prefix(dce:=<http://purl.org/dc/elements/1.1/>)
Prefix(owl:=<http://www.w3.org/2002/07/owl#>)
Prefix(pmd:=<https://w3id.org/pmd/co/>)
Prefix(rdf:=<http://www.w3.org/1999/02/22-rdf-syntax-ns#>)
Prefix(xml:=<http://www.w3.org/XML/1998/namespace>)
Prefix(xsd:=<http://www.w3.org/2001/XMLSchema#>)
Prefix(rdfs:=<http://www.w3.org/2000/01/rdf-schema#>)
Prefix(dcterms:=<http://purl.org/dc/terms/>)


Ontology(<https://w3id.org/pmd/ao/tto/>
Import(<https://w3id.org/pmd/ao/tto/imports/pmdco_import.owl>)
Annotation(dcterms:contributor "https://orcid.org/0000-0003-1649-6832")
Annotation(dcterms:creator <https://orcid.org/0000-0001-7192-7143>)
Annotation(dcterms:creator <https://orcid.org/0000-0002-3717-7104>)
Annotation(dcterms:creator <https://orcid.org/0000-0002-7094-5371>)
Annotation(dcterms:creator <https://orcid.org/0000-0002-9014-2920>)
Annotation(dcterms:creator <https://orcid.org/0000-0003-4971-3645>)
Annotation(dcterms:description "Dies ist die PMD-Ontologie für Zugversuche (Tensile Test Ontology – TTO), die auf der Grundlage der Prüfnorm \"ISO 6892-1: Metallische Werkstoffe – Zugversuche – Teil 1: Prüfverfahren bei Raumtemperatur\" entwickelt wurde.

Die TTO wurde im Rahmen des PMD-Projekts entwickelt. Die TTO bietet Konzeptualisierungen, die für die Beschreibung von Zugversuchen und entsprechenden Daten gemäß der jeweiligen Prüfnorm gültig sind. Durch die Verwendung der TTO zur Speicherung von Zugversuchsdaten sind alle Daten gut strukturiert und basieren auf einem gemeinsamen Vokabular, das von einer Expertengruppe vereinbart wurde (Erzeugung von FAIRen-Daten), was zu einer verbesserten Dateninteroperabilität führen wird. Durch den Import der PMD Core Ontology (PMDco) wird die Interoperabilität von Zugprüfungsdaten verbessert und die Abfrage in Kombination mit anderen Aspekten und Daten aus dem breiten Feld der Materialwissenschaft und Werkstofftechnik (MSE) erleichtert."@de)
Annotation(dcterms:description "This is thePMD ontology of the tensile test (Tensile Test Ontology - TTO) as developed on the basis of the test standard ISO 6892-1: Metallic materials - Tensile Testing - Part 1: Method of test at room temperature.

The TTO was developed in the frame of the PMD project. The TTO provides conceptualizations valid for the description of tensile tests and corresponding data in accordance with the respective test standard. By using TTO for storing tensile test data, all data will be well structured and based on a common vocabulary agreed on by an expert group (generation of FAIR data) which will lead to enhanced data interoperability. Due to the import of the PMD core ontology (PMDco), the interoperability of tensile test data is enhanced and querying in combination with other aspects and data within the broad field of material science and engineering (MSE) is facilitated."@en)
Annotation(dcterms:license <http://creativecommons.org/licenses/by/4.0/>)
Annotation(dcterms:title "Tensile Test Ontology (TTO)")

Declaration(Class(:TTO_0000000))
Declaration(Class(:TTO_0000001))
Declaration(Class(:TTO_0000002))
Declaration(Class(:TTO_0000004))
Declaration(Class(:TTO_0000005))
Declaration(Class(:TTO_0000006))
Declaration(Class(:TTO_0000007))
Declaration(Class(:TTO_0000008))
Declaration(Class(:TTO_0000009))
Declaration(Class(:TTO_0000010))
Declaration(Class(:TTO_0000011))
Declaration(Class(:TTO_0000012))
Declaration(Class(:TTO_0000013))
Declaration(Class(:TTO_0000014))
Declaration(Class(:TTO_0000015))
Declaration(Class(:TTO_0000016))
Declaration(Class(:TTO_0000017))
Declaration(Class(:TTO_0000018))
Declaration(Class(:TTO_0000019))
Declaration(Class(:TTO_0000020))
Declaration(Class(:TTO_0000021))
Declaration(Class(:TTO_0000022))
Declaration(Class(:TTO_0000023))
Declaration(Class(:TTO_0000024))
Declaration(Class(:TTO_0000025))
Declaration(Class(:TTO_0000026))
Declaration(Class(:TTO_0000027))
Declaration(Class(:TTO_0000028))
Declaration(Class(:TTO_0000029))
Declaration(Class(:TTO_0000030))
Declaration(Class(:TTO_0000031))
Declaration(Class(:TTO_0000032))
Declaration(Class(:TTO_0000033))
Declaration(Class(:TTO_0000034))
Declaration(Class(:TTO_0000035))
Declaration(Class(:TTO_0000036))
Declaration(Class(:TTO_0000037))
Declaration(Class(:TTO_0000038))
Declaration(Class(:TTO_0000039))
Declaration(Class(:TTO_0000040))
Declaration(Class(:TTO_0000041))
Declaration(Class(:TTO_0000042))
Declaration(Class(:TTO_0000043))
Declaration(Class(:TTO_0000044))
Declaration(Class(:TTO_0000045))
Declaration(Class(:TTO_0000046))
Declaration(Class(:TTO_0000047))
Declaration(Class(:TTO_0000048))
Declaration(Class(:TTO_0000049))
Declaration(Class(:TTO_0000050))
Declaration(Class(:TTO_0000051))
Declaration(Class(:TTO_0000052))
Declaration(Class(:TTO_0000053))
Declaration(Class(:TTO_0000054))
Declaration(Class(:TTO_0000055))
Declaration(Class(:TTO_0000056))
Declaration(Class(:TTO_0000057))
Declaration(Class(:TTO_0000058))
Declaration(Class(:TTO_0000059))
Declaration(Class(:TTO_0000060))
Declaration(ObjectProperty(pmd:relatesTo))
Declaration(DataProperty(<http://www.w3.org/ns/prov#value>))
Declaration(AnnotationProperty(dcterms:description))
Declaration(AnnotationProperty(dcterms:license))
Declaration(AnnotationProperty(dcterms:title))
Declaration(AnnotationProperty(pmd:definitionSource))
Declaration(AnnotationProperty(pmd:symbol))




############################
#   Classes
############################

# Class: :TTO_0000000 (Förderungsrolle)

AnnotationAssertion(rdfs:label :TTO_0000000 "Förderungsrolle"@de)
AnnotationAssertion(rdfs:label :TTO_0000000 "funder role"@en)
AnnotationAssertion(<http://www.w3.org/2004/02/skos/core#definition> :TTO_0000000 "A funder role is a role that describes the capacity in which a party provides financial support to a project or initiative. This role is realized when the party participates in the project specifically as a source of funding, regardless of other potential involvements."@en)
AnnotationAssertion(<http://www.w3.org/2004/02/skos/core#definition> :TTO_0000000 "Eine Förderungsrolle (Rolle einer fördernden Partei) ist eine Rolle, die die Funktion beschreibt, in der eine Partei finanzielle Unterstützung für ein Projekt oder eine Initiative bereitstellt. Diese Rolle wird verwirklicht, wenn die Partei speziell als Geldgeber am Projekt teilnimmt, unabhängig von anderen möglichen Beteiligungen."@de)
SubClassOf(:TTO_0000000 <http://purl.obolibrary.org/obo/BFO_0000023>)

# Class: :TTO_0000001 (Höchstkraft der Kraftmessdose)

AnnotationAssertion(rdfs:label :TTO_0000001 "Höchstkraft der Kraftmessdose"@de)
AnnotationAssertion(rdfs:label :TTO_0000001 "load cell maximum force"@en)
AnnotationAssertion(<http://www.w3.org/2004/02/skos/core#definition> :TTO_0000001 "Die Maximalkraft bezeichnet die größte Kraft, die eine Kraftmessdose bei einem Zugversuch zuverlässig und ohne bleibende Beschädigung messen kann. Sie definiert die obere Belastungsgrenze des Sensors, oberhalb derer Messfehler, plastische Verformungen oder ein Ausfall des Messsystems auftreten können."@de)
AnnotationAssertion(<http://www.w3.org/2004/02/skos/core#definition> :TTO_0000001 "The maximum force is the highest force that a load cell can reliably measure during a tensile test without permanent damage. It defines the upper load limit of the sensor, beyond which measurement errors, plastic deformation, or failure of the system may occur."@en)
SubClassOf(:TTO_0000001 pmd:PMD_0020200)

# Class: :TTO_0000002 (Diameter)

AnnotationAssertion(rdfs:isDefinedBy :TTO_0000002 <https://w3id.org/pmd/ao/tto>)
AnnotationAssertion(rdfs:label :TTO_0000002 "Diameter"@en)
AnnotationAssertion(rdfs:label :TTO_0000002 "Durchmesser"@de)
AnnotationAssertion(rdfs:seeAlso :TTO_0000002 <https://w3id.org/pmd/co/2.0.8/Diameter>)
AnnotationAssertion(<http://www.w3.org/2004/02/skos/core#definition> :TTO_0000002 "Die Länge einer geraden Linie durch den Mittelpunkt eines Objekts oder Raums."@de)
AnnotationAssertion(<http://www.w3.org/2004/02/skos/core#definition> :TTO_0000002 "The length of a straight line through the center of an object or space."@en)
AnnotationAssertion(pmd:definitionSource :TTO_0000002 "“Diameter.” Merriam-Webster.com Dictionary, Merriam-Webster, https://www.merriam-webster.com/dictionary/diameter. Accessed 5 Dec. 2022.")
SubClassOf(:TTO_0000002 pmd:PMD_0040001)

# Class: :TTO_0000004 (Verlängerung)

AnnotationAssertion(rdfs:isDefinedBy :TTO_0000004 <https://w3id.org/pmd/ao/tto>)
AnnotationAssertion(rdfs:label :TTO_0000004 "Elongation"@en)
AnnotationAssertion(rdfs:label :TTO_0000004 "Verlängerung"@de)
AnnotationAssertion(rdfs:seeAlso :TTO_0000004 <https://w3id.org/pmd/tto/Elongation>)
AnnotationAssertion(<http://www.w3.org/2004/02/skos/core#definition> :TTO_0000004 "Zunahme der Anfangsmesslänge zu einem beliebigen Zeitpunkt während des Versuchs"@de)
AnnotationAssertion(<http://www.w3.org/2004/02/skos/core#definition> :TTO_0000004 "increase in the original gauge length at any moment during the test"@en)
AnnotationAssertion(pmd:definitionSource :TTO_0000004 "DIN EN ISO 6892-1:2019"@en)
SubClassOf(:TTO_0000004 pmd:PMD_0040001)
SubClassOf(:TTO_0000004 ObjectSomeValuesFrom(pmd:relatesTo :TTO_0000028))

# Class: :TTO_0000005 (Extension)

AnnotationAssertion(<http://purl.obolibrary.org/obo/IAO_0000114> :TTO_0000005 <http://purl.obolibrary.org/obo/IAO_0000428>)
AnnotationAssertion(rdfs:comment :TTO_0000005 "Dimensional analysis: L
Unit (e.g. SI): mm"@en)
AnnotationAssertion(rdfs:comment :TTO_0000005 "Hinweis: Die Dehnung kann mit verschiedenen Kanälen gemessen werden (z. B. bei Verwendung von einem oder zwei Dehnungsmesserkanälen); in der Regel wird als Dehnungswert der mittlere Durchschnittswert der beteiligten Kanäle angegeben, falls zutreffend.

Hinweis: Die optische Längenänderungsmessung kann eine besondere Methode der Datenspeicherung erfordern."@de)
AnnotationAssertion(rdfs:comment :TTO_0000005 "Note: The extension might be measured using different channels (e.g. when using one or two extensometer channels); usually, the mean average value of involved channels is given as extension value, if applicable.

Note: Optical extensometry may require a specific data storage method."@en)
AnnotationAssertion(rdfs:isDefinedBy :TTO_0000005 <https://w3id.org/pmd/ao/tto>)
AnnotationAssertion(rdfs:label :TTO_0000005 "Extension"@en)
AnnotationAssertion(rdfs:label :TTO_0000005 "Verlängerung (der Extensometer-Messlänge)"@de)
AnnotationAssertion(rdfs:seeAlso :TTO_0000005 <https://w3id.org/pmd/co/2.0.8/Extension>)
AnnotationAssertion(<http://www.w3.org/2004/02/skos/core#definition> :TTO_0000005 "Increase in the extensometer gauge length at any moment during a test"@en)
AnnotationAssertion(<http://www.w3.org/2004/02/skos/core#definition> :TTO_0000005 "Zunahme der Extensometer-Messlänge zu einem beliebigen Zeitpunkt eines Versuchs"@de)
AnnotationAssertion(pmd:definitionSource :TTO_0000005 "DIN EN ISO 6892-1:2019")
SubClassOf(:TTO_0000005 pmd:PMD_0000848)

# Class: :TTO_0000006 (Thickness)

AnnotationAssertion(rdfs:isDefinedBy :TTO_0000006 <https://w3id.org/pmd/ao/tto>)
AnnotationAssertion(rdfs:label :TTO_0000006 "Dicke"@de)
AnnotationAssertion(rdfs:label :TTO_0000006 "Thickness"@en)
AnnotationAssertion(rdfs:seeAlso :TTO_0000006 <https://w3id.org/pmd/co/2.0.8/Thickness>)
AnnotationAssertion(<http://www.w3.org/2004/02/skos/core#definition> :TTO_0000006 "Diese Klasse beschreibt das gemessene Maß in einer Richtung eines Prüfkörpers."@de)
AnnotationAssertion(<http://www.w3.org/2004/02/skos/core#definition> :TTO_0000006 "This class describes the measured dimension in one direction of a test piece."@en)
SubClassOf(:TTO_0000006 pmd:PMD_0040001)

# Class: :TTO_0000007 (Area)

AnnotationAssertion(rdfs:isDefinedBy :TTO_0000007 <https://w3id.org/pmd/ao/tto>)
AnnotationAssertion(rdfs:label :TTO_0000007 "Area"@en)
AnnotationAssertion(rdfs:label :TTO_0000007 "Fläche"@de)
AnnotationAssertion(rdfs:seeAlso :TTO_0000007 <https://w3id.org/pmd/co/2.0.8/Area>)
AnnotationAssertion(<http://www.w3.org/2004/02/skos/core#definition> :TTO_0000007 "Die Ausdehnung oder Messung einer Fläche."@de)
AnnotationAssertion(<http://www.w3.org/2004/02/skos/core#definition> :TTO_0000007 "The extent or measurement of a surface."@en)
SubClassOf(:TTO_0000007 pmd:PMD_0020132)

# Class: :TTO_0000008 (Form)

AnnotationAssertion(rdfs:isDefinedBy :TTO_0000008 <https://w3id.org/pmd/ao/tto>)
AnnotationAssertion(rdfs:label :TTO_0000008 "Form"@de)
AnnotationAssertion(rdfs:label :TTO_0000008 "Shape"@en)
AnnotationAssertion(rdfs:seeAlso :TTO_0000008 <https://w3id.org/pmd/tto/Shape>)
AnnotationAssertion(<http://www.w3.org/2004/02/skos/core#definition> :TTO_0000008 "Das sichtbare Ausstattungsmerkmal (räumliche Form oder Kontur) eines bestimmten Objektes oder einer Art von Objekt."@de)
AnnotationAssertion(<http://www.w3.org/2004/02/skos/core#definition> :TTO_0000008 "The visible makeup characteristic (spatial form or contour) of a particular item or kind of item."@en)
AnnotationAssertion(pmd:definitionSource :TTO_0000008 "“Shape.” Merriam-Webster.com Dictionary, Merriam-Webster, https://www.merriam-webster.com/dictionary/shape. Accessed 13 Jan. 2023.")
SubClassOf(:TTO_0000008 pmd:PMD_0020148)

# Class: :TTO_0000009 (Streckgrenze)

AnnotationAssertion(rdfs:isDefinedBy :TTO_0000009 <https://w3id.org/pmd/ao/tto>)
AnnotationAssertion(rdfs:label :TTO_0000009 "Streckgrenze"@de)
AnnotationAssertion(rdfs:label :TTO_0000009 "Yield Strength"@en)
AnnotationAssertion(rdfs:seeAlso :TTO_0000009 <https://w3id.org/pmd/tto/YieldStrength>)
AnnotationAssertion(<http://www.w3.org/2004/02/skos/core#definition> :TTO_0000009 "Wenn der metallische Werkstoff diese Eigenschaft aufweist: die Spannung zu einem bestimmten Zeitpunkt während des Versuchs bei dem eine plastische Verformung ohne Zunahme der Kraft auftritt"@de)
AnnotationAssertion(<http://www.w3.org/2004/02/skos/core#definition> :TTO_0000009 "when the metallic material exhibits a yield phenomenon, stress corresponding to the point reached during the test at which plastic deformation occurs without any increase in the force"@en)
AnnotationAssertion(pmd:definitionSource :TTO_0000009 "DIN EN ISO 6892-1:2019"@en)
SubClassOf(:TTO_0000009 pmd:PMD_0000952)

# Class: :TTO_0000010 (Width)

AnnotationAssertion(rdfs:isDefinedBy :TTO_0000010 <https://w3id.org/pmd/ao/tto>)
AnnotationAssertion(rdfs:label :TTO_0000010 "Breite"@de)
AnnotationAssertion(rdfs:label :TTO_0000010 "Width"@en)
AnnotationAssertion(rdfs:seeAlso :TTO_0000010 <https://w3id.org/pmd/co/2.0.8/Width>)
AnnotationAssertion(<http://www.w3.org/2004/02/skos/core#definition> :TTO_0000010 "Diese Klasse beschreibt eine horizontale Messung eines Objekts, die im rechten Winkel zur Länge des Objekts vorgenommen wird."@de)
AnnotationAssertion(<http://www.w3.org/2004/02/skos/core#definition> :TTO_0000010 "This class describes a horizontal measurement of an object taken at right angles to the length of the object."@en)
AnnotationAssertion(pmd:definitionSource :TTO_0000010 <https://www.merriam-webster.com/dictionary/width>)
SubClassOf(:TTO_0000010 pmd:PMD_0040001)

# Class: :TTO_0000011 (Änderung der transversalen Dimension)

AnnotationAssertion(rdfs:isDefinedBy :TTO_0000011 <https://w3id.org/pmd/ao/tto>)
AnnotationAssertion(rdfs:label :TTO_0000011 "Change Of Transverse Dimension"@en)
AnnotationAssertion(rdfs:label :TTO_0000011 "Änderung der transversalen Dimension"@de)
AnnotationAssertion(rdfs:seeAlso :TTO_0000011 <https://w3id.org/pmd/tto/ChangeOfTransverseDimension>)
AnnotationAssertion(<http://www.w3.org/2004/02/skos/core#definition> :TTO_0000011 "Dieses Konzept beschreibt eine Variation der Abmessungen eines Prüfkörpers in Bezug auf seine Querachse, die sich auf seine Querschnittsfläche auswirkt und möglicherweise während eines Zugversuchs auftritt. Das Verhältnis der wahren plastischen Breitendehnung und der wahren plastischen Dickendehnung in einem in uniaxialem Zug beanspruchten Prüfkörper (vertikale Anisotropie) kann anhand dieser Information berechnet werden."@de)
AnnotationAssertion(<http://www.w3.org/2004/02/skos/core#definition> :TTO_0000011 "This concept describes a variation in the dimension of a test piece referring to its transversal axis affecting its cross-sectional area that may potentially occur during a tensile test. The ratio of the true plastic strain in width and the true plastic strain in thickness in a test piece loaded in uniaxial tension (vertical anisotropy) may be calculated using this information."@en)
AnnotationAssertion(pmd:definitionSource :TTO_0000011 "DIN EN ISO 10113:2021-06")
SubClassOf(:TTO_0000011 pmd:PMD_0040001)

# Class: :TTO_0000012 (Querschnittsfläche)

AnnotationAssertion(rdfs:isDefinedBy :TTO_0000012 <https://w3id.org/pmd/tto>)
AnnotationAssertion(rdfs:label :TTO_0000012 "Cross Section Area"@en)
AnnotationAssertion(rdfs:label :TTO_0000012 "Querschnittsfläche"@de)
AnnotationAssertion(rdfs:seeAlso :TTO_0000012 <https://w3id.org/pmd/co/2.0.8/CrossSectionArea>)
AnnotationAssertion(<http://www.w3.org/2004/02/skos/core#definition> :TTO_0000012 "Die Querschnittsfläche ist die Fläche eines Schnittes oder eines rechtwinklig geschnittenen oder gebrochenen Stücks eines Objektes in Bezug auf eine Achse."@de)
AnnotationAssertion(<http://www.w3.org/2004/02/skos/core#definition> :TTO_0000012 "The cross section area is an area of a cutting or piece of an object cut off or broken at right angles or related to an axis."@en)
AnnotationAssertion(pmd:definitionSource :TTO_0000012 <https://www.merriam-webster.com/dictionary/cross%20section>)
SubClassOf(:TTO_0000012 :TTO_0000007)

# Class: :TTO_0000013 (Crosshead Separation)

AnnotationAssertion(rdfs:comment :TTO_0000013 "Dimensional analysis: L
Unit (e.g. SI): mm"@en)
AnnotationAssertion(rdfs:isDefinedBy :TTO_0000013 <https://w3id.org/pmd/ao/tto>)
AnnotationAssertion(rdfs:label :TTO_0000013 "Crosshead Separation"@en)
AnnotationAssertion(rdfs:label :TTO_0000013 "Querhaupttrennung"@de)
AnnotationAssertion(rdfs:seeAlso :TTO_0000013 <https://w3id.org/pmd/tto/CrossheadSeparation>)
AnnotationAssertion(<http://www.w3.org/2004/02/skos/core#definition> :TTO_0000013 "Dieses Konzept beschreibt die Verschiebung der Traverse einer Zugprüfmaschine."@de)
AnnotationAssertion(<http://www.w3.org/2004/02/skos/core#definition> :TTO_0000013 "This concept describes the displacement of the crossheads of a tensile testing machine."@en)
AnnotationAssertion(pmd:definitionSource :TTO_0000013 "DIN EN ISO 6892-1:2019"@en)
SubClassOf(:TTO_0000013 pmd:PMD_0040001)

# Class: :TTO_0000014 (Crosshead Separation Rate)

AnnotationAssertion(rdfs:isDefinedBy :TTO_0000014 <https://w3id.org/pmd/ao/tto>)
AnnotationAssertion(rdfs:label :TTO_0000014 "Crosshead Separation Rate"@en)
AnnotationAssertion(rdfs:label :TTO_0000014 "Traversengeschwindigkeit"@de)
AnnotationAssertion(rdfs:seeAlso :TTO_0000014 <https://w3id.org/pmd/tto/CrossheadSeparationRate>)
AnnotationAssertion(<http://www.w3.org/2004/02/skos/core#definition> :TTO_0000014 "Traversenweg je Zeiteinheit"@de)
AnnotationAssertion(<http://www.w3.org/2004/02/skos/core#definition> :TTO_0000014 "displacement of the crossheads per time"@en)
AnnotationAssertion(pmd:definitionSource :TTO_0000014 "DIN EN ISO 6892-1:2019"@en)
AnnotationAssertion(pmd:symbol :TTO_0000014 "v_c"@en)
SubClassOf(:TTO_0000014 :TTO_0000025)

# Class: :TTO_0000015 (End-Probendurchmesser)

AnnotationAssertion(rdfs:isDefinedBy :TTO_0000015 <https://w3id.org/pmd/tto>)
AnnotationAssertion(rdfs:label :TTO_0000015 "Diameter After Fracture"@en)
AnnotationAssertion(rdfs:label :TTO_0000015 "End-Probendurchmesser"@de)
AnnotationAssertion(rdfs:seeAlso :TTO_0000015 <https://w3id.org/pmd/tto/DiameterAfterFracture>)
AnnotationAssertion(<http://www.w3.org/2004/02/skos/core#definition> :TTO_0000015 "Die Länge einer geraden Linie durch den Mittelpunkt eines Objekts (Zugprüfstücks), gemessen nach einem Bruch, der während einer Prüfung aufgetreten ist."@de)
AnnotationAssertion(<http://www.w3.org/2004/02/skos/core#definition> :TTO_0000015 "The length of a straight line through the center of an object (tensile test piece) as measured after a fracture occured during a test."@en)
SubClassOf(:TTO_0000015 :TTO_0000002)

# Class: :TTO_0000016 (Abgeschätzte Dehngeschwindigkeit Über Die Parallele Länge)

AnnotationAssertion(rdfs:isDefinedBy :TTO_0000016 <https://w3id.org/pmd/ao/tto>)
AnnotationAssertion(rdfs:label :TTO_0000016 "Abgeschätzte Dehngeschwindigkeit Über Die Parallele Länge"@de)
AnnotationAssertion(rdfs:label :TTO_0000016 "Estimated Strain Rate Over The Parallel Length"@en)
AnnotationAssertion(rdfs:seeAlso :TTO_0000016 <https://w3id.org/pmd/tto/EstimatedStrainRateOverTheParallelLength>)
AnnotationAssertion(<http://www.w3.org/2004/02/skos/core#definition> :TTO_0000016 "Zunahme der Dehnung über die parallele Länge der Probe je Zeiteinheit, basierend auf der Traversengeschwindigkeit und der parallelen Länge der Probe"@de)
AnnotationAssertion(<http://www.w3.org/2004/02/skos/core#definition> :TTO_0000016 "value of the increase of strain over the parallel length of the test piece per time based on the crosshead separation rate and the parallel length of the test piece"@en)
AnnotationAssertion(pmd:definitionSource :TTO_0000016 "DIN EN ISO 6892-1:2019"@en)
AnnotationAssertion(pmd:symbol :TTO_0000016 "e^._L_c"@en)
SubClassOf(:TTO_0000016 :TTO_0000025)

# Class: :TTO_0000017 (Extensometer Gauge Length)

AnnotationAssertion(rdfs:isDefinedBy :TTO_0000017 <https://w3id.org/pmd/ao/tto>)
AnnotationAssertion(rdfs:label :TTO_0000017 "Extensometer Gauge Length"@en)
AnnotationAssertion(rdfs:label :TTO_0000017 "Extensometer-Messlänge"@de)
AnnotationAssertion(rdfs:seeAlso :TTO_0000017 <https://w3id.org/pmd/tto/ExtensometerGaugeLength>)
AnnotationAssertion(<http://www.w3.org/2004/02/skos/core#definition> :TTO_0000017 "Anfangsmesslänge des Dehnungsaufnehmers (Extensometer), die zum Messen der Verlängerung benutzt wird

Anmerkung: Für die Bestimmung mehrerer Eigenschaften, die (teilweise oder vollständig) von der Verlängerung abhängig sind, z. B. R_p, A_e oder A_g, ist die Verwendung eines Extensometers zwingend erforderlich."@de)
AnnotationAssertion(<http://www.w3.org/2004/02/skos/core#definition> :TTO_0000017 "initial gauge length of the extensometer used for measurement of extension

Note: For the determination of several properties which are based (partly or complete) on extension, e. g. R_p, A_e or A_g, the use of an extensometer is mandatory."@en)
AnnotationAssertion(pmd:definitionSource :TTO_0000017 "DIN EN ISO 6892-1:2019"@en)
AnnotationAssertion(pmd:symbol :TTO_0000017 "L_e"@en)
SubClassOf(:TTO_0000017 :TTO_0000019)

# Class: :TTO_0000018 (Final Gauge Length After Fracture)

AnnotationAssertion(rdfs:isDefinedBy :TTO_0000018 <https://w3id.org/pmd/ao/tto>)
AnnotationAssertion(rdfs:label :TTO_0000018 "Final Gauge Length After Fracture"@en)
AnnotationAssertion(rdfs:label :TTO_0000018 "Messlänge nach dem Bruch"@de)
AnnotationAssertion(rdfs:seeAlso :TTO_0000018 <https://w3id.org/pmd/tto/FinalGaugeLengthAfterFracture>)
AnnotationAssertion(<http://www.w3.org/2004/02/skos/core#definition> :TTO_0000018 "Länge zwischen den Marken zur Kennzeichnung der Messlänge auf der Probe, die nach dem Bruch bei Raumtemperatur gemessen wird, nachdem die beiden Probenbruchstücke sorgfältig so zusammengefügt wurden, dass ihre Achsen in einer Geraden liegen"@de)
AnnotationAssertion(<http://www.w3.org/2004/02/skos/core#definition> :TTO_0000018 "length between gauge length marks on the test piece measured after rupture, at room temperature, the two pieces having been carefully fitted back together so that their axes lie in a straight line"@en)
AnnotationAssertion(pmd:definitionSource :TTO_0000018 "DIN EN ISO 6892-1:2019"@en)
AnnotationAssertion(pmd:symbol :TTO_0000018 "L_u"@en)
SubClassOf(:TTO_0000018 :TTO_0000019)

# Class: :TTO_0000019 (Messlänge)

AnnotationAssertion(rdfs:isDefinedBy :TTO_0000019 <https://w3id.org/pmd/ao/tto>)
AnnotationAssertion(rdfs:label :TTO_0000019 "Gauge Length"@en)
AnnotationAssertion(rdfs:label :TTO_0000019 "Messlänge"@de)
AnnotationAssertion(rdfs:seeAlso :TTO_0000019 <https://w3id.org/pmd/tto/GaugeLength>)
AnnotationAssertion(<http://www.w3.org/2004/02/skos/core#definition> :TTO_0000019 "Länge des parallelen Teils der Probe, an dem zu einem beliebigen Zeitpunkt während des Versuchs die Verlängerung gemessen wird"@de)
AnnotationAssertion(<http://www.w3.org/2004/02/skos/core#definition> :TTO_0000019 "length of the parallel portion of the test piece on which elongation is measured at any moment during the test"@en)
AnnotationAssertion(pmd:definitionSource :TTO_0000019 "DIN EN ISO 6892-1:2019"@en)
AnnotationAssertion(pmd:symbol :TTO_0000019 "L"@en)
SubClassOf(:TTO_0000019 pmd:PMD_0040001)

# Class: :TTO_0000020 (Gauge Length Marks)

AnnotationAssertion(<http://purl.obolibrary.org/obo/IAO_0000114> :TTO_0000020 <http://purl.obolibrary.org/obo/IAO_0000428>)
AnnotationAssertion(rdfs:isDefinedBy :TTO_0000020 <https://w3id.org/pmd/ao/tto>)
AnnotationAssertion(rdfs:label :TTO_0000020 "Gauge Length Marks"@en)
AnnotationAssertion(rdfs:label :TTO_0000020 "Messlängenmarkierungen"@de)
AnnotationAssertion(rdfs:seeAlso :TTO_0000020 <https://w3id.org/pmd/tto/GaugeLengthMarks>)
AnnotationAssertion(<http://www.w3.org/2004/02/skos/core#definition> :TTO_0000020 "Dieses Konzept wird verwendet, um die sichtbaren Markierungen zu beschreiben, die in der Regel während eines Zugversuchs zur Messung der Dehnung an den Prüfkörpern angebracht werden."@de)
AnnotationAssertion(<http://www.w3.org/2004/02/skos/core#definition> :TTO_0000020 "This concept is used to describe the visible markers usually attached to test pieces during a tensile test for elongation / extension measurements."@en)
SubClassOf(:TTO_0000020 pmd:PMD_0000602)

# Class: :TTO_0000021 (Geometry Shape)

AnnotationAssertion(<http://purl.obolibrary.org/obo/IAO_0000114> :TTO_0000021 <http://purl.obolibrary.org/obo/IAO_0000428>)
AnnotationAssertion(rdfs:isDefinedBy :TTO_0000021 <https://w3id.org/pmd/tto>)
AnnotationAssertion(rdfs:label :TTO_0000021 "Geometrische Form"@de)
AnnotationAssertion(rdfs:label :TTO_0000021 "Geometry Shape"@en)
AnnotationAssertion(rdfs:seeAlso :TTO_0000021 <https://w3id.org/pmd/tto/GeometryShape>)
AnnotationAssertion(<http://www.w3.org/2004/02/skos/core#definition> :TTO_0000021 "Dieses Konzept beschreibt die geometrischen Abmessungen und das Erscheinungsbild (Form und Abmaße) einer Probe, eines Prüfkörpers oder eines Prüfstücks, wie sie üblicherweise durch eine entsprechende Norm definiert sind. Dementsprechend ist der angegebene Formwert in Übereinstimmung mit der definierenden Norm anzugeben, z. B. \"Zugprüfstück Form 1 gemäß Anhang B\"."@de)
AnnotationAssertion(<http://www.w3.org/2004/02/skos/core#definition> :TTO_0000021 "This concept describes the geometric dimensions and appearance (shape and dimensions) of a sample, specimen, or test piece as usually defined by a corresponding standard. Accordingly, the shape value given is in accordance with the defining standard, e.g., ‘tensile test piece shape 1 in accordance with annex B’."@en)
AnnotationAssertion(pmd:definitionSource :TTO_0000021 "DIN EN ISO 6892-1:2019"@en)
SubClassOf(:TTO_0000021 :TTO_0000008)

# Class: :TTO_0000022 (untere Streckgrenze)

AnnotationAssertion(rdfs:isDefinedBy :TTO_0000022 <https://w3id.org/pmd/ao/tto>)
AnnotationAssertion(rdfs:label :TTO_0000022 "Lower Yield Strength"@en)
AnnotationAssertion(rdfs:label :TTO_0000022 "untere Streckgrenze"@de)
AnnotationAssertion(rdfs:seeAlso :TTO_0000022 <https://w3id.org/pmd/tto/LowerYieldStrength>)
AnnotationAssertion(<http://www.w3.org/2004/02/skos/core#definition> :TTO_0000022 "kleinste Spannung während des plastischen Fließens, wobei Einschwingerscheinungen nicht berücksichtigt werden"@de)
AnnotationAssertion(<http://www.w3.org/2004/02/skos/core#definition> :TTO_0000022 "lowest value of stress during plastic yielding, ignoring any initial transient effects"@en)
AnnotationAssertion(pmd:definitionSource :TTO_0000022 "DIN EN ISO 6892-1:2019"@en)
AnnotationAssertion(pmd:symbol :TTO_0000022 "R_eL"@en)
SubClassOf(:TTO_0000022 :TTO_0000009)

# Class: :TTO_0000023 (Höchstkraft)

AnnotationAssertion(rdfs:isDefinedBy :TTO_0000023 <https://w3id.org/pmd/tto>)
AnnotationAssertion(rdfs:label :TTO_0000023 "Höchstkraft"@de)
AnnotationAssertion(rdfs:label :TTO_0000023 "Maximum Force"@en)
AnnotationAssertion(rdfs:seeAlso :TTO_0000023 <https://w3id.org/pmd/tto/MaximumForce>)
AnnotationAssertion(<http://www.w3.org/2004/02/skos/core#definition> :TTO_0000023 "Bei Werkstoffen, die kein diskontinuierliches Fließen zeigen: größte Kraft, der die Probe während des Versuchs standhält

Bei Werkstoffen, die ein diskontinuierliches Fließen zeigen: größte Kraft, der die Probe während des Versuchs nach dem Beginn der Verfestigung standhält

Anmerkung: Für Werkstoffe, die ein diskontinuierliches Fließen zeigen, aber keine Verfestigung erzielt werden kann, ist die Höchstkraft nicht definiert
."@de)
AnnotationAssertion(<http://www.w3.org/2004/02/skos/core#definition> :TTO_0000023 "For materials displaying no discontinuous yielding: highest force that the test piece withstands during the test

For materials displaying discontinuous yielding: highest force that the test piece withstands during the test after the beginning of work-hardening

Note: For materials which display discontinuous yielding, but where no work-hardening can be established, the maximum force is not defined."@en)
AnnotationAssertion(pmd:definitionSource :TTO_0000023 "DIN EN ISO 6892-1:2019"@en)
SubClassOf(:TTO_0000023 pmd:PMD_0020200)

# Class: :TTO_0000024 (Minimum cross-sectional area after fracture)

AnnotationAssertion(rdfs:comment :TTO_0000024 "Symbol: S_u")
AnnotationAssertion(rdfs:isDefinedBy :TTO_0000024 <https://w3id.org/pmd/ao/tto>)
AnnotationAssertion(rdfs:label :TTO_0000024 "Kleinster Querschnitt nach dem Bruch"@de)
AnnotationAssertion(rdfs:label :TTO_0000024 "Minimum cross-sectional area after fracture"@en)
AnnotationAssertion(rdfs:seeAlso :TTO_0000024 <https://w3id.org/pmd/tto/MinimumCrossSectionalAreaAfterFracture>)
AnnotationAssertion(<http://www.w3.org/2004/02/skos/core#definition> :TTO_0000024 "Dieses Konzept beschreibt die kleinste Querschnittsfläche des Zugprüfkörers, die nach dem Bruch infolge der aufgebrachten Zugkraft erhalten wird.

Anmerkung: Sie wird in der Regel senkrecht zur Richtung der aufgebrachten Kraft gemessen und dient zur Berechnung der technischen Spannung während der Prüfung.

Anmerkung: Es wird empfohlen, den Anfangsquerschnitt innerhalb der parallelen Länge mit einer Genauigkeit von ±2 % zu messen. Bei runden Prüfkörpern mit kleinem Durchmesser oder Prüfkörpern mit anderen Querschnittsgeometrien ist es jedoch möglicherweise nicht möglich, den Anfangsquerschnitt innerhalb der parallelen Länge mit einer Genauigkeit von ±2 % zu messen."@de)
AnnotationAssertion(<http://www.w3.org/2004/02/skos/core#definition> :TTO_0000024 "This concept describes the smallest cross-sectional area of the tensile test piece observed after it has fractured under the applied tensile force.

Note: It is typically measured perpendicular to the direction of the applied force and is used to calculate engineering stress during the test.

Note: It is recommended to measure the original cross-sectional area of the parallel length to an accuracy of ±2 %. However, measuring the original cross-sectional area of the parallel length with an accuracy of ±2 % on small diameter round test pieces, or test pieces with other cross-sectional geometries, may not be possible."@en)
AnnotationAssertion(pmd:definitionSource :TTO_0000024 "DIN EN ISO 6892-1:2019")
SubClassOf(:TTO_0000024 :TTO_0000012)
SubClassOf(:TTO_0000024 ObjectUnionOf(ObjectIntersectionOf(ObjectSomeValuesFrom(pmd:relatesTo :TTO_0000056) ObjectSomeValuesFrom(pmd:relatesTo :TTO_0000060)) ObjectSomeValuesFrom(pmd:relatesTo :TTO_0000015)))

# Class: :TTO_0000025 (Movement Quality)

AnnotationAssertion(rdfs:isDefinedBy :TTO_0000025 <https://w3id.org/pmd/ao/tto>)
AnnotationAssertion(rdfs:label :TTO_0000025 "Bewegungsqualität"@de)
AnnotationAssertion(rdfs:label :TTO_0000025 "Movement Quality"@en)
AnnotationAssertion(rdfs:seeAlso :TTO_0000025 <https://w3id.org/pmd/tto/MovementQuality>)
AnnotationAssertion(<http://www.w3.org/2004/02/skos/core#definition> :TTO_0000025 "A movement quality is a physical quality that inheres in a material entity and represents a property of the entity's motion or change of position over time."@en)
AnnotationAssertion(<http://www.w3.org/2004/02/skos/core#definition> :TTO_0000025 "Eine Bewegungsqualität ist eine physikalische Qualität, die einer materiellen Entität innewohnt und eine Eigenschaft der Bewegung oder Positionsänderung der Entität im Laufe der Zeit darstellt."@de)
SubClassOf(:TTO_0000025 :TTO_0000042)

# Class: :TTO_0000026 (Anfangsquerschnitt innerhalb der parallelen Länge)

AnnotationAssertion(rdfs:comment :TTO_0000026 "Symbol: S_o")
AnnotationAssertion(rdfs:isDefinedBy :TTO_0000026 <https://w3id.org/pmd/ao/tto>)
AnnotationAssertion(rdfs:label :TTO_0000026 "Anfangsquerschnitt innerhalb der parallelen Länge"@de)
AnnotationAssertion(rdfs:label :TTO_0000026 "Original cross-sectional area of the parallel length"@en)
AnnotationAssertion(rdfs:seeAlso :TTO_0000026 <https://w3id.org/pmd/tto/OriginalCrossSectionalArea>)
AnnotationAssertion(<http://www.w3.org/2004/02/skos/core#definition> :TTO_0000026 "Dieses Konzept beschreibt die initiale Querschnittsfläche des Zugprüfkörpers entlang seiner parallelen Länge, bevor eine Verformung auftritt."@de)
AnnotationAssertion(<http://www.w3.org/2004/02/skos/core#definition> :TTO_0000026 "This concept describes the initial area of the tensile test piece before any deformation occurs."@en)
AnnotationAssertion(pmd:definitionSource :TTO_0000026 "DIN EN ISO 6892-1:2019")
SubClassOf(:TTO_0000026 :TTO_0000012)
SubClassOf(:TTO_0000026 ObjectUnionOf(ObjectIntersectionOf(ObjectSomeValuesFrom(pmd:relatesTo :TTO_0000029) ObjectSomeValuesFrom(pmd:relatesTo :TTO_0000030)) ObjectSomeValuesFrom(pmd:relatesTo :TTO_0000027)))

# Class: :TTO_0000027 (Original Diameter)

AnnotationAssertion(rdfs:isDefinedBy :TTO_0000027 <https://w3id.org/pmd/tto>)
AnnotationAssertion(rdfs:label :TTO_0000027 "Anfangs-Probendurchmesser"@de)
AnnotationAssertion(rdfs:label :TTO_0000027 "Original Diameter"@en)
AnnotationAssertion(rdfs:seeAlso :TTO_0000027 <https://w3id.org/pmd/tto/OriginalDiameter>)
AnnotationAssertion(<http://www.w3.org/2004/02/skos/core#definition> :TTO_0000027 "Die Länge einer geraden Linie durch den Mittelpunkt eines Objekts (Zugprüfkörpers), die vor einer Prüfung gemessen wird."@de)
AnnotationAssertion(<http://www.w3.org/2004/02/skos/core#definition> :TTO_0000027 "The length of a straight line through the center of an object (tensile test piece) as measured prior to a tensile test."@en)
AnnotationAssertion(pmd:definitionSource :TTO_0000027 "DIN EN ISO 6892-1:2019"@en)
SubClassOf(:TTO_0000027 :TTO_0000002)

# Class: :TTO_0000028 (Original Gauge Length)

AnnotationAssertion(rdfs:isDefinedBy :TTO_0000028 <https://w3id.org/pmd/ao/tto>)
AnnotationAssertion(rdfs:label :TTO_0000028 "Anfangsmesslänge"@de)
AnnotationAssertion(rdfs:label :TTO_0000028 "Original Gauge Length"@en)
AnnotationAssertion(rdfs:seeAlso :TTO_0000028 <https://w3id.org/pmd/tto/OriginalGaugeLength>)
AnnotationAssertion(<http://www.w3.org/2004/02/skos/core#definition> :TTO_0000028 "Länge zwischen den Marken zur Kennzeichnung der Messlänge auf der Probe, die vor dem Versuch bei Raumtemperatur gemessen wird"@de)
AnnotationAssertion(<http://www.w3.org/2004/02/skos/core#definition> :TTO_0000028 "length between gauge length marks on the test piece measured at room temperature before the test"@en)
AnnotationAssertion(pmd:definitionSource :TTO_0000028 "DIN EN ISO 6892-1:2019"@en)
AnnotationAssertion(pmd:symbol :TTO_0000028 "L_o"@en)
SubClassOf(:TTO_0000028 :TTO_0000019)

# Class: :TTO_0000029 (Anfangs-Dicke)

AnnotationAssertion(rdfs:isDefinedBy :TTO_0000029 <https://w3id.org/pmd/ao/tto>)
AnnotationAssertion(rdfs:label :TTO_0000029 "Anfangs-Dicke"@de)
AnnotationAssertion(rdfs:label :TTO_0000029 "Original Thickness"@en)
AnnotationAssertion(rdfs:seeAlso :TTO_0000029 <https://w3id.org/pmd/tto/OriginalThickness>)
AnnotationAssertion(<http://www.w3.org/2004/02/skos/core#definition> :TTO_0000029 "Diese Entität beschreibt die gemessene Dimension in einer Richtung eines Prüfstücks, wie sie vor der Prüfung gemessen wurde."@de)
AnnotationAssertion(<http://www.w3.org/2004/02/skos/core#definition> :TTO_0000029 "This entity describes the measured dimension in one direction of a test piece, as measured before the test."@en)
SubClassOf(:TTO_0000029 :TTO_0000006)

# Class: :TTO_0000030 (Original Width)

AnnotationAssertion(rdfs:isDefinedBy :TTO_0000030 <https://w3id.org/pmd/ao/tto>)
AnnotationAssertion(rdfs:label :TTO_0000030 "Anfangs-Breite"@de)
AnnotationAssertion(rdfs:label :TTO_0000030 "Original Width"@en)
AnnotationAssertion(rdfs:seeAlso :TTO_0000030 <https://w3id.org/pmd/tto/OriginalWidth>)
AnnotationAssertion(<http://www.w3.org/2004/02/skos/core#definition> :TTO_0000030 "Diese Entität beschreibt eine horizontale Messung eines Objekts (Prüfkörpers) im rechten Winkel zur Länge des Objekts (Prüfkörpers), wie sie vor einer Prüfung gemessen wird."@de)
AnnotationAssertion(<http://www.w3.org/2004/02/skos/core#definition> :TTO_0000030 "This entity describes a horizontal measurement of an object (test piece) taken at right angles to the length of the object (test piece), as measured before a test."@en)
SubClassOf(:TTO_0000030 :TTO_0000010)

# Class: :TTO_0000031 (Parallele Länge)

AnnotationAssertion(rdfs:isDefinedBy :TTO_0000031 <https://w3id.org/pmd/ao/tto>)
AnnotationAssertion(rdfs:label :TTO_0000031 "Parallel Length"@en)
AnnotationAssertion(rdfs:label :TTO_0000031 "Parallele Länge"@de)
AnnotationAssertion(rdfs:seeAlso :TTO_0000031 <https://w3id.org/pmd/tto/ParallelLength>)
AnnotationAssertion(<http://www.w3.org/2004/02/skos/core#definition> :TTO_0000031 "Länge des parallelen reduzierten Querschnitts der Probe

Anmerkung: Bei unbearbeiteten Proben tritt an die Stelle der parallelen Länge der Abstand zwischen den Einspannungen."@de)
AnnotationAssertion(<http://www.w3.org/2004/02/skos/core#definition> :TTO_0000031 "length of the parallel reduced section of the test piece

Note: The concept of parallel length is replaced by the concept of distance between grips for unmachined test pieces."@en)
AnnotationAssertion(pmd:definitionSource :TTO_0000031 "DIN EN ISO 6892-1:2019"@en)
AnnotationAssertion(pmd:symbol :TTO_0000031 "L_c"@en)
SubClassOf(:TTO_0000031 pmd:PMD_0040001)

# Class: :TTO_0000032 (Dehnung)

AnnotationAssertion(rdfs:isDefinedBy :TTO_0000032 <https://w3id.org/pmd/ao/tto>)
AnnotationAssertion(rdfs:label :TTO_0000032 "Dehnung"@de)
AnnotationAssertion(rdfs:label :TTO_0000032 "Percentage Elongation"@en)
AnnotationAssertion(rdfs:seeAlso :TTO_0000032 <https://w3id.org/pmd/tto/PercentageElongation>)
AnnotationAssertion(<http://www.w3.org/2004/02/skos/core#definition> :TTO_0000032 "Verlängerung, angegeben in Prozent, bezogen auf die Anfangsmesslänge"@de)
AnnotationAssertion(<http://www.w3.org/2004/02/skos/core#definition> :TTO_0000032 "elongation expressed as a percentage of the original gauge length"@en)
AnnotationAssertion(pmd:definitionSource :TTO_0000032 "DIN EN ISO 6892-1:2019"@en)
SubClassOf(:TTO_0000032 :TTO_0000004)
SubClassOf(:TTO_0000032 ObjectSomeValuesFrom(pmd:relatesTo :TTO_0000028))

# Class: :TTO_0000033 (Bruchdehnung)

AnnotationAssertion(rdfs:isDefinedBy :TTO_0000033 <https://w3id.org/pmd/ao/tto>)
AnnotationAssertion(rdfs:label :TTO_0000033 "Bruchdehnung"@de)
AnnotationAssertion(rdfs:label :TTO_0000033 "Percentage Elongation After Fracture"@en)
AnnotationAssertion(rdfs:seeAlso :TTO_0000033 <https://w3id.org/pmd/tto/PercentageElongationAfterFracture>)
AnnotationAssertion(<http://www.w3.org/2004/02/skos/core#definition> :TTO_0000033 "bleibende Verlängerung der Messlänge nach dem Bruch (L_u − L_o), angegeben in Prozent, bezogen auf die Anfangsmesslänge"@de)
AnnotationAssertion(<http://www.w3.org/2004/02/skos/core#definition> :TTO_0000033 "permanent elongation of the gauge length after fracture (L_u − L_o), expressed as a percentage of the original gauge length"@en)
AnnotationAssertion(pmd:definitionSource :TTO_0000033 "DIN EN ISO 6892-1:2019"@en)
AnnotationAssertion(pmd:symbol :TTO_0000033 "A"@en)
SubClassOf(:TTO_0000033 :TTO_0000004)
SubClassOf(:TTO_0000033 ObjectSomeValuesFrom(pmd:relatesTo :TTO_0000028))

# Class: :TTO_0000034 (Extensometer-Dehnung)

AnnotationAssertion(rdfs:isDefinedBy :TTO_0000034 <https://w3id.org/pmd/tto>)
AnnotationAssertion(rdfs:label :TTO_0000034 "Extensometer-Dehnung"@de)
AnnotationAssertion(rdfs:label :TTO_0000034 "Percentage Extension"@en)
AnnotationAssertion(rdfs:seeAlso :TTO_0000034 <https://w3id.org/pmd/co/2.0.8/PercentageExtension>)
AnnotationAssertion(<http://www.w3.org/2004/02/skos/core#altLabel> :TTO_0000034 "(engineering) strain"@en)
AnnotationAssertion(<http://www.w3.org/2004/02/skos/core#altLabel> :TTO_0000034 "technische Dehnung"@de)
AnnotationAssertion(<http://www.w3.org/2004/02/skos/core#definition> :TTO_0000034 "extension expressed as a percentage of the extensometer gauge length

Note: The percentage extension is commonly called engineering strain."@en)
AnnotationAssertion(<http://www.w3.org/2004/02/skos/core#definition> :TTO_0000034 "in Prozent angegebene Verlängerung der Extensometer-Messlänge

Anmerkung: Die Extensometer-Dehnung wird oftmals auch als technische Dehnung bezeichnet.")
AnnotationAssertion(pmd:definitionSource :TTO_0000034 "DIN EN ISO 6892-1:2019")
SubClassOf(:TTO_0000034 :TTO_0000005)
SubClassOf(:TTO_0000034 ObjectSomeValuesFrom(pmd:relatesTo :TTO_0000017))

# Class: :TTO_0000035 (Percentage Permanent Elongation)

AnnotationAssertion(rdfs:isDefinedBy :TTO_0000035 <https://w3id.org/pmd/ao/tto>)
AnnotationAssertion(rdfs:label :TTO_0000035 "Bleibende Dehnung"@de)
AnnotationAssertion(rdfs:label :TTO_0000035 "Percentage Permanent Elongation"@en)
AnnotationAssertion(rdfs:seeAlso :TTO_0000035 <https://w3id.org/pmd/tto/PercentagePermanentElongation>)
AnnotationAssertion(<http://www.w3.org/2004/02/skos/core#definition> :TTO_0000035 "Zunahme der Anfangsmesslänge einer Probe nach Entfernen einer festgelegten Zugspannung, angegeben in Prozent, bezogen auf die Anfangsmesslänge"@de)
AnnotationAssertion(<http://www.w3.org/2004/02/skos/core#definition> :TTO_0000035 "increase in the original gauge length of a test piece after removal of a specified stress, expressed as a percentage of the original gauge length"@en)
AnnotationAssertion(pmd:definitionSource :TTO_0000035 "DIN EN ISO 6892-1:2019"@en)
SubClassOf(:TTO_0000035 :TTO_0000004)
SubClassOf(:TTO_0000035 ObjectSomeValuesFrom(pmd:relatesTo :TTO_0000028))

# Class: :TTO_0000036 (Bleibende Extensometer-Dehnung)

AnnotationAssertion(rdfs:isDefinedBy :TTO_0000036 <https://w3id.org/pmd/ao/tto>)
AnnotationAssertion(rdfs:label :TTO_0000036 "Bleibende Extensometer-Dehnung"@de)
AnnotationAssertion(rdfs:label :TTO_0000036 "Percentage Permanent Extension"@en)
AnnotationAssertion(rdfs:seeAlso :TTO_0000036 <https://w3id.org/pmd/tto/PercentagePermanentExtension>)
AnnotationAssertion(<http://www.w3.org/2004/02/skos/core#definition> :TTO_0000036 "Vergrößerung der Extensometer-Messlänge nach Entfernen einer festgelegten, auf die Probe aufgebrachten Zugspannung, angegeben in Prozent, bezogen auf die Extensometer-Messlänge"@de)
AnnotationAssertion(<http://www.w3.org/2004/02/skos/core#definition> :TTO_0000036 "increase in the extensometer gauge length, after removal of a specified stress from the test piece, expressed as a percentage of the extensometer gauge length"@en)
AnnotationAssertion(pmd:definitionSource :TTO_0000036 "DIN EN ISO 6892-1:2019"@en)
SubClassOf(:TTO_0000036 :TTO_0000005)
SubClassOf(:TTO_0000036 ObjectSomeValuesFrom(pmd:relatesTo :TTO_0000017))

# Class: :TTO_0000037 (Plastische Extensometer-Dehnung bei Höchstkraft)

AnnotationAssertion(rdfs:isDefinedBy :TTO_0000037 <https://w3id.org/pmd/ao/tto>)
AnnotationAssertion(rdfs:label :TTO_0000037 "Percentage Plastic Extension At Maximum Force"@en)
AnnotationAssertion(rdfs:label :TTO_0000037 "Plastische Extensometer-Dehnung bei Höchstkraft"@de)
AnnotationAssertion(rdfs:seeAlso :TTO_0000037 <https://w3id.org/pmd/tto/PercentagePlasticExtensionAtMaximumForce>)
AnnotationAssertion(<http://www.w3.org/2004/02/skos/core#definition> :TTO_0000037 "plastic extension at maximum force, expressed as a percentage of the extensometer gauge length"@en)
AnnotationAssertion(<http://www.w3.org/2004/02/skos/core#definition> :TTO_0000037 "plastische Verlängerung der Extensometer-Messlänge bei Höchstkraft, angegeben in Prozent, bezogen auf die Extensometer-Messlänge"@de)
AnnotationAssertion(pmd:definitionSource :TTO_0000037 "DIN EN ISO 6892-1:2019"@en)
AnnotationAssertion(pmd:symbol :TTO_0000037 "A_g"@en)
SubClassOf(:TTO_0000037 :TTO_0000005)
SubClassOf(:TTO_0000037 ObjectIntersectionOf(ObjectSomeValuesFrom(pmd:relatesTo :TTO_0000017) ObjectSomeValuesFrom(pmd:relatesTo :TTO_0000023)))

# Class: :TTO_0000038 (Percentage Reduction Of Area)

AnnotationAssertion(rdfs:isDefinedBy :TTO_0000038 <https://w3id.org/pmd/ao/tto>)
AnnotationAssertion(rdfs:label :TTO_0000038 "Brucheinschnürung"@de)
AnnotationAssertion(rdfs:label :TTO_0000038 "Percentage Reduction Of Area"@en)
AnnotationAssertion(rdfs:seeAlso :TTO_0000038 <https://w3id.org/pmd/tto/PercentageReductionOfArea>)
AnnotationAssertion(<http://www.w3.org/2004/02/skos/core#definition> :TTO_0000038 "größte während des Versuchs aufgetretene Änderung des Querschnitts (S_o − S_u), angegeben in Prozent, bezogen auf den Anfangsquerschnitt S_o"@de)
AnnotationAssertion(<http://www.w3.org/2004/02/skos/core#definition> :TTO_0000038 "maximum change in cross-sectional area which has occurred during the test (S_o − S_u), expressed as a percentage of the original cross-sectional area, S_o"@en)
AnnotationAssertion(pmd:definitionSource :TTO_0000038 "DIN EN ISO 6892-1:2019"@en)
AnnotationAssertion(pmd:symbol :TTO_0000038 "Z")
SubClassOf(:TTO_0000038 :TTO_0000049)
SubClassOf(:TTO_0000038 ObjectIntersectionOf(ObjectSomeValuesFrom(pmd:relatesTo :TTO_0000024) ObjectSomeValuesFrom(pmd:relatesTo :TTO_0000026)))

# Class: :TTO_0000039 (Percentage Total Extension At Fracture)

AnnotationAssertion(rdfs:isDefinedBy :TTO_0000039 <https://w3id.org/pmd/ao/tto>)
AnnotationAssertion(rdfs:label :TTO_0000039 "Gesamte Extensometer-Dehnung beim Bruch"@de)
AnnotationAssertion(rdfs:label :TTO_0000039 "Percentage Total Extension At Fracture"@en)
AnnotationAssertion(rdfs:seeAlso :TTO_0000039 <https://w3id.org/pmd/tto/PercentageTotalExtensionAtFracture>)
AnnotationAssertion(<http://www.w3.org/2004/02/skos/core#definition> :TTO_0000039 "gesamte Verlängerung (elastische plus plastische Verlängerung) der Extensometer-Messlänge beim Bruch, angegeben in Prozent, bezogen auf die Extensometer-Messlänge"@de)
AnnotationAssertion(<http://www.w3.org/2004/02/skos/core#definition> :TTO_0000039 "total extension (elastic extension plus plastic extension) at the moment of fracture, expressed as a percentage of the extensometer gauge length"@en)
AnnotationAssertion(pmd:definitionSource :TTO_0000039 "DIN EN ISO 6892-1:2019"@en)
AnnotationAssertion(pmd:symbol :TTO_0000039 "A_t"@en)
SubClassOf(:TTO_0000039 :TTO_0000005)
SubClassOf(:TTO_0000039 ObjectSomeValuesFrom(pmd:relatesTo :TTO_0000017))

# Class: :TTO_0000040 (Gesamte Extensometer-Dehnung bei Höchstkraft)

AnnotationAssertion(rdfs:isDefinedBy :TTO_0000040 <https://w3id.org/pmd/ao/tto>)
AnnotationAssertion(rdfs:label :TTO_0000040 "Gesamte Extensometer-Dehnung bei Höchstkraft"@de)
AnnotationAssertion(rdfs:label :TTO_0000040 "Percentage Total Extension At Maximum Force"@en)
AnnotationAssertion(rdfs:seeAlso :TTO_0000040 <https://w3id.org/pmd/tto/PercentageTotalExtensionAtMaximumForce>)
AnnotationAssertion(<http://www.w3.org/2004/02/skos/core#definition> :TTO_0000040 "gesamte Verlängerung (elastische plus plastische Verlängerung) der Extensometer-Messlänge bei Höchstkraft, angegeben in Prozent, bezogen auf die Extensometer-Messlänge"@de)
AnnotationAssertion(<http://www.w3.org/2004/02/skos/core#definition> :TTO_0000040 "total extension (elastic extension plus plastic extension) at maximum force, expressed as a percentage of the extensometer gauge length"@en)
AnnotationAssertion(pmd:definitionSource :TTO_0000040 "DIN EN ISO 6892-1:2019"@en)
AnnotationAssertion(pmd:symbol :TTO_0000040 "A_gt"@en)
SubClassOf(:TTO_0000040 :TTO_0000005)
SubClassOf(:TTO_0000040 ObjectIntersectionOf(ObjectSomeValuesFrom(pmd:relatesTo :TTO_0000017) ObjectSomeValuesFrom(pmd:relatesTo :TTO_0000023)))

# Class: :TTO_0000041 (Percentage Yield Point Extension)

AnnotationAssertion(rdfs:isDefinedBy :TTO_0000041 <https://w3id.org/pmd/ao/tto>)
AnnotationAssertion(rdfs:label :TTO_0000041 "Percentage Yield Point Extension"@en)
AnnotationAssertion(rdfs:label :TTO_0000041 "Streckgrenzen-Extensometer-Dehnung"@de)
AnnotationAssertion(rdfs:seeAlso :TTO_0000041 <https://w3id.org/pmd/tto/PercentageYieldPointExtension>)
AnnotationAssertion(<http://www.w3.org/2004/02/skos/core#definition> :TTO_0000041 "Bei Werkstoffen, die ein diskontinuierliches Fließen zeigen: Verlängerung der Extensometer-Messlänge zwischen dem Beginn örtlichen Fließens und dem Einsetzen gleichmäßiger Verfestigung, angegeben in Prozent, bezogen auf die Extensometer-Messlänge"@de)
AnnotationAssertion(<http://www.w3.org/2004/02/skos/core#definition> :TTO_0000041 "For discontinuous yielding materials: extension between the start of yielding and the start of uniform work-hardening, expressed as a percentage of the extensometer gauge length"@en)
AnnotationAssertion(pmd:definitionSource :TTO_0000041 "DIN EN ISO 6892-1:2019"@en)
AnnotationAssertion(pmd:symbol :TTO_0000041 "A_e"@en)
SubClassOf(:TTO_0000041 :TTO_0000005)

# Class: :TTO_0000042 (Physical Quality)

AnnotationAssertion(rdfs:isDefinedBy :TTO_0000042 <https://w3id.org/pmd/ao/tto>)
AnnotationAssertion(rdfs:label :TTO_0000042 "Physical Quality"@en)
AnnotationAssertion(rdfs:label :TTO_0000042 "Physikalische Qualität"@de)
AnnotationAssertion(rdfs:seeAlso :TTO_0000042 <https://w3id.org/pmd/tto/PhysicalQuality>)
AnnotationAssertion(<http://www.w3.org/2004/02/skos/core#definition> :TTO_0000042 "A physical quality is a quality that inheres in a material entity and represents a measurable or observable property related to its physical state."@en)
AnnotationAssertion(<http://www.w3.org/2004/02/skos/core#definition> :TTO_0000042 "Eine physikalische Qualität ist eine Eigenschaft, die einer materiellen Einheit innewohnt und eine messbare oder beobachtbare Eigenschaft darstellt, die mit ihrem physikalischen Zustand zusammenhängt."@de)
SubClassOf(:TTO_0000042 <http://purl.obolibrary.org/obo/BFO_0000019>)

# Class: :TTO_0000043 (Dehngrenze)

AnnotationAssertion(rdfs:isDefinedBy :TTO_0000043 <https://w3id.org/pmd/ao/tto>)
AnnotationAssertion(rdfs:label :TTO_0000043 "Dehngrenze"@de)
AnnotationAssertion(rdfs:label :TTO_0000043 "Proof Strength"@en)
AnnotationAssertion(rdfs:seeAlso :TTO_0000043 <https://w3id.org/pmd/tto/ProofStrength>)
AnnotationAssertion(<http://www.w3.org/2004/02/skos/core#definition> :TTO_0000043 "Spannung, bei der ein bestimmter Dehnungswert gleich einem bestimmten Prozentsatz der Messlänge des Dehnungsmessers ist"@de)
AnnotationAssertion(<http://www.w3.org/2004/02/skos/core#definition> :TTO_0000043 "stress at which the a specific extension value is equal to a specified percentage of the extensometer gauge length"@en)
SubClassOf(:TTO_0000043 pmd:PMD_0000952)

# Class: :TTO_0000044 (Proof Strength Plastic Extension)

AnnotationAssertion(rdfs:isDefinedBy :TTO_0000044 <https://w3id.org/pmd/ao/tto>)
AnnotationAssertion(rdfs:label :TTO_0000044 "Dehngrenze bei plastischer Extensometer-Dehnung"@de)
AnnotationAssertion(rdfs:label :TTO_0000044 "Proof Strength Plastic Extension"@en)
AnnotationAssertion(rdfs:seeAlso :TTO_0000044 <https://w3id.org/pmd/tto/ProofStrengthPlasticExtension>)
AnnotationAssertion(<http://www.w3.org/2004/02/skos/core#definition> :TTO_0000044 "Spannung, bei der die plastische Extensometer-Dehnung einem vorgegebenen Prozentanteil der Extensometer-Messlänge entspricht

Anmerkung: Der Index wird durch den Zahlenwert ergänzt, der den vorgegebenen Zahlenwert der plastischen Extensometer-Dehnung in Prozent angibt, z. B. R_p_0,2."@de)
AnnotationAssertion(<http://www.w3.org/2004/02/skos/core#definition> :TTO_0000044 "stress at which the plastic extension is equal to a specified percentage of the extensometer gauge length

Note: A suffix is added to the subscript to indicate the prescribed percentage, e.g. R_p_0.2.

Source: ISO 6892-1:2019"@en)
AnnotationAssertion(pmd:definitionSource :TTO_0000044 "DIN EN ISO 6892-1:2019"@en)
AnnotationAssertion(pmd:symbol :TTO_0000044 "R_p"@en)
SubClassOf(:TTO_0000044 :TTO_0000043)

# Class: :TTO_0000045 (Dehngrenze bei gesamter Extensometer-Dehnung)

AnnotationAssertion(rdfs:isDefinedBy :TTO_0000045 <https://w3id.org/pmd/ao/tto>)
AnnotationAssertion(rdfs:label :TTO_0000045 "Dehngrenze bei gesamter Extensometer-Dehnung"@de)
AnnotationAssertion(rdfs:label :TTO_0000045 "Proof Strength Total Extension"@en)
AnnotationAssertion(rdfs:seeAlso :TTO_0000045 <https://w3id.org/pmd/tto/ProofStrengthTotalExtension>)
AnnotationAssertion(<http://www.w3.org/2004/02/skos/core#definition> :TTO_0000045 "Spannung, bei der die gesamte Extensometer-Dehnung (elastische und plastische Extensometer-Dehnung) einem vorgegebenen Prozentanteil der Extensometer-Messlänge entspricht

Anmerkung: Der Index wird durch den Zahlenwert ergänzt, der den vorgegebenen Zahlenwert der gesamten Extensometer-Dehnung in Prozent angibt, z. B. R_t_0,5."@de)
AnnotationAssertion(<http://www.w3.org/2004/02/skos/core#definition> :TTO_0000045 "stress at which total extension (elastic extension plus plastic extension) is equal to a specified percentage of the extensometer gauge length

Note: A suffix is added to the subscript to indicate the prescribed percentage, e.g. R_t_0.5."@en)
AnnotationAssertion(pmd:definitionSource :TTO_0000045 "DIN EN ISO 6892-1:2019"@en)
AnnotationAssertion(pmd:symbol :TTO_0000045 "R_t"@en)
SubClassOf(:TTO_0000045 :TTO_0000043)
SubClassOf(:TTO_0000045 ObjectSomeValuesFrom(pmd:relatesTo :TTO_0000017))

# Class: :TTO_0000046 (Dehngrenze bei plastischer Extensometer-Dehnung Rp01)

AnnotationAssertion(rdfs:isDefinedBy :TTO_0000046 <https://w3id.org/pmd/ao/tto>)
AnnotationAssertion(rdfs:label :TTO_0000046 "Dehngrenze bei plastischer Extensometer-Dehnung Rp01"@de)
AnnotationAssertion(rdfs:label :TTO_0000046 "Proof Strength Plastic Extension Rp01"@en)
AnnotationAssertion(rdfs:seeAlso :TTO_0000046 <https://w3id.org/pmd/tto/Rp01>)
AnnotationAssertion(<http://www.w3.org/2004/02/skos/core#definition> :TTO_0000046 "Spannung bei einer plastischen Extensometer-Dehnung, die 0,1 Prozent der Extensometer-Messlänge entspricht"@de)
AnnotationAssertion(<http://www.w3.org/2004/02/skos/core#definition> :TTO_0000046 "stress at which the plastic extension is equal to 0.1 percent of the extensometer gauge length"@en)
AnnotationAssertion(pmd:definitionSource :TTO_0000046 "DIN EN ISO 6892-1:2019"@en)
AnnotationAssertion(pmd:symbol :TTO_0000046 "R_p_0.1"@en)
SubClassOf(:TTO_0000046 :TTO_0000044)

# Class: :TTO_0000047 (Dehngrenze bei plastischer Extensometer-Dehnung Rp02)

AnnotationAssertion(rdfs:isDefinedBy :TTO_0000047 <https://w3id.org/pmd/ao/tto>)
AnnotationAssertion(rdfs:label :TTO_0000047 "Dehngrenze bei plastischer Extensometer-Dehnung Rp02"@de)
AnnotationAssertion(rdfs:label :TTO_0000047 "Proof Strength Plastic Extension Rp02"@en)
AnnotationAssertion(rdfs:seeAlso :TTO_0000047 <https://w3id.org/pmd/tto/Rp02>)
AnnotationAssertion(<http://www.w3.org/2004/02/skos/core#definition> :TTO_0000047 "Spannung bei einer plastischen Extensometer-Dehnung, die 0,2 Prozent der Extensometer-Messlänge entspricht"@de)
AnnotationAssertion(<http://www.w3.org/2004/02/skos/core#definition> :TTO_0000047 "stress at which the plastic extension is equal to 0.2 percent of the extensometer gauge length"@en)
AnnotationAssertion(pmd:definitionSource :TTO_0000047 "DIN EN ISO 6892-1:2019"@en)
AnnotationAssertion(pmd:symbol :TTO_0000047 "R_p_0.2"@en)
SubClassOf(:TTO_0000047 :TTO_0000044)

# Class: :TTO_0000048 (3D Geometrie)

AnnotationAssertion(rdfs:isDefinedBy :TTO_0000048 <https://w3id.org/pmd/tto>)
AnnotationAssertion(rdfs:label :TTO_0000048 "3D Geometrie"@de)
AnnotationAssertion(rdfs:label :TTO_0000048 "Shape 3D"@en)
AnnotationAssertion(rdfs:seeAlso :TTO_0000048 <https://w3id.org/pmd/tto/Shape3D>)
AnnotationAssertion(<http://www.w3.org/2004/02/skos/core#definition> :TTO_0000048 "A shape 3D is a geometry shape that exists in three dimensions, having length, width, and height, and can be defined by its spatial properties such as volume and surface area."@en)
AnnotationAssertion(<http://www.w3.org/2004/02/skos/core#definition> :TTO_0000048 "Eine 3D Geometrie ist eine geometrische Form, die in drei Dimensionen existiert, mit Länge, Breite und Höhe, und die durch ihre räumlichen Eigenschaften wie Volumen und Oberfläche definiert werden kann."@de)
AnnotationAssertion(<http://www.w3.org/2004/02/skos/core#example> :TTO_0000048 "Beispiele sind Formen wie Würfel, Kugeln und Pyramiden."@de)
AnnotationAssertion(<http://www.w3.org/2004/02/skos/core#example> :TTO_0000048 "Examples include shapes like cubes, spheres, and pyramids."@en)
SubClassOf(:TTO_0000048 :TTO_0000021)

# Class: :TTO_0000049 (Size Relation)

AnnotationAssertion(<http://purl.obolibrary.org/obo/IAO_0000114> :TTO_0000049 <http://purl.obolibrary.org/obo/IAO_0000428>)
AnnotationAssertion(rdfs:isDefinedBy :TTO_0000049 <https://w3id.org/pmd/ao/tto>)
AnnotationAssertion(rdfs:label :TTO_0000049 "Größenrelation"@de)
AnnotationAssertion(rdfs:label :TTO_0000049 "Size Relation"@en)
AnnotationAssertion(rdfs:seeAlso :TTO_0000049 <https://w3id.org/pmd/tto/SizeRelation>)
SubClassOf(:TTO_0000049 :TTO_0000042)

# Class: :TTO_0000050 (Steigung des elastischen Bereichs)

AnnotationAssertion(rdfs:isDefinedBy :TTO_0000050 <https://w3id.org/pmd/ao/tto>)
AnnotationAssertion(rdfs:label :TTO_0000050 "Slope Of The Elastic Part"@en)
AnnotationAssertion(rdfs:label :TTO_0000050 "Steigung des elastischen Bereichs"@de)
AnnotationAssertion(rdfs:seeAlso :TTO_0000050 <https://w3id.org/pmd/tto/SlopeOfTheElasticPart>)
AnnotationAssertion(<http://www.w3.org/2004/02/skos/core#definition> :TTO_0000050 "Dieses Konzept beschreibt den Wert der Steigung des ersten linear ansteigenden Teils (\"elastischer Teil\") in der bei einem Zugversuch erhaltenen Spannungs-Dehnungs-Kurve. Im elastischen Teil der Spannungs-Dehnungs-Kurve muss der Wert der Steigung nicht unbedingt dem Elastizitätsmodul entsprechen. Dieser Wert kann mit dem Wert des Elastizitätsmoduls (nur) sehr gut übereinstimmen, wenn optimale Bedingungen herrschten."@de)
AnnotationAssertion(<http://www.w3.org/2004/02/skos/core#definition> :TTO_0000050 "This concept describes the value of the slope of the first linear increasing part (‘elastic part’) in the stress-percentage extension curve obtained during a tensile test. In the elastic part of the stress‐percentage extension curve, the value of the slope may not necessarily represent the modulus of elasticity. This value may closely agree with the value of the modulus of elasticity if optimal conditions were used."@en)
AnnotationAssertion(pmd:definitionSource :TTO_0000050 "DIN EN ISO 6892-1:2019"@en)
SubClassOf(:TTO_0000050 pmd:PMD_0000618)

# Class: :TTO_0000051 (Dehngeschwindigkeit)

AnnotationAssertion(rdfs:isDefinedBy :TTO_0000051 <https://w3id.org/pmd/ao/tto>)
AnnotationAssertion(rdfs:label :TTO_0000051 "Dehngeschwindigkeit"@de)
AnnotationAssertion(rdfs:label :TTO_0000051 "Strain Rate"@en)
AnnotationAssertion(rdfs:seeAlso :TTO_0000051 <https://w3id.org/pmd/tto/StrainRate>)
AnnotationAssertion(<http://www.w3.org/2004/02/skos/core#definition> :TTO_0000051 "Zunahme der mit einem Extensometer in der Extensometer-Messlänge gemessenen Dehnung je Zeiteinheit"@de)
AnnotationAssertion(<http://www.w3.org/2004/02/skos/core#definition> :TTO_0000051 "increase of strain, measured with an extensometer, in extensometer gauge length, per time"@en)
AnnotationAssertion(pmd:definitionSource :TTO_0000051 "DIN EN ISO 6892-1:2019"@en)
AnnotationAssertion(pmd:symbol :TTO_0000051 "e^._L_e"@en)
SubClassOf(:TTO_0000051 :TTO_0000025)

# Class: :TTO_0000052 (Stress Rate)

AnnotationAssertion(rdfs:isDefinedBy :TTO_0000052 <https://w3id.org/pmd/ao/tto>)
AnnotationAssertion(rdfs:label :TTO_0000052 "Spannungsgeschwindigkeit"@de)
AnnotationAssertion(rdfs:label :TTO_0000052 "Stress Rate"@en)
AnnotationAssertion(rdfs:seeAlso :TTO_0000052 <https://w3id.org/pmd/tto/StressRate>)
AnnotationAssertion(<http://www.w3.org/2004/02/skos/core#definition> :TTO_0000052 "Zunahme der Spannung je Zeiteinheit

Anmerkung: Die Spannungsgeschwindigkeit wird nur im elastischen Bereich des Versuchs verwendet."@de)
AnnotationAssertion(<http://www.w3.org/2004/02/skos/core#definition> :TTO_0000052 "increase of stress per time

Note: Stress rate is only used in the elastic part of the test."@en)
AnnotationAssertion(pmd:definitionSource :TTO_0000052 "DIN EN ISO 6892-1:2019"@en)
AnnotationAssertion(pmd:symbol :TTO_0000052 "R"@en)
SubClassOf(:TTO_0000052 :TTO_0000025)

# Class: :TTO_0000053 (Tensile Strength)

AnnotationAssertion(<http://purl.obolibrary.org/obo/IAO_0000114> :TTO_0000053 <http://purl.obolibrary.org/obo/IAO_0000428>)
AnnotationAssertion(rdfs:isDefinedBy :TTO_0000053 <https://w3id.org/pmd/ao/tto>)
AnnotationAssertion(rdfs:label :TTO_0000053 "Tensile Strength"@en)
AnnotationAssertion(rdfs:label :TTO_0000053 "Zugfestigkeit"@de)
AnnotationAssertion(rdfs:seeAlso :TTO_0000053 <https://w3id.org/pmd/tto/TensileStrength>)
AnnotationAssertion(<http://www.w3.org/2004/02/skos/core#definition> :TTO_0000053 "Spannung, die der Höchstkraft entspricht"@de)
AnnotationAssertion(<http://www.w3.org/2004/02/skos/core#definition> :TTO_0000053 "stress corresponding to the maximum force"@en)
AnnotationAssertion(pmd:definitionSource :TTO_0000053 "DIN EN ISO 6892-1:2019"@en)
AnnotationAssertion(pmd:symbol :TTO_0000053 "R_m"@en)
SubClassOf(:TTO_0000053 pmd:PMD_0000952)

# Class: :TTO_0000054 (Zugversuchsmethode)

AnnotationAssertion(rdfs:isDefinedBy :TTO_0000054 <https://w3id.org/pmd/tto>)
AnnotationAssertion(rdfs:label :TTO_0000054 "Tensile Test Method"@en)
AnnotationAssertion(rdfs:label :TTO_0000054 "Zugversuchsmethode"@de)
AnnotationAssertion(rdfs:seeAlso :TTO_0000054 <https://w3id.org/pmd/tto/TensileTestMethod>)
AnnotationAssertion(<http://www.w3.org/2004/02/skos/core#definition> :TTO_0000054 "A tensile test method is a plan specification that prescribes the execution of a controlled experiment designed to determine the mechanical properties of a material under uniaxial tensile loading. The plan specifies procedural steps, conditions, and measurement criteria to assess properties such as ultimate tensile strength, yield strength, and elongation at break."@en)
AnnotationAssertion(<http://www.w3.org/2004/02/skos/core#definition> :TTO_0000054 "Eine Zugversuchsmethode ist eine Planspezifikation, die die Durchführung eines kontrollierten Versuchs zur Bestimmung der mechanischen Eigenschaften eines Materials unter einachsiger Zugbelastung vorschreibt. Der Plan legt Verfahrensschritte, Bedingungen und Messkriterien fest, um Eigenschaften wie die Zugfestigkeit, die Streckgrenze und die Bruchdehnung zu bestimmen."@de)
SubClassOf(:TTO_0000054 pmd:PMD_0000003)

# Class: :TTO_0000055 (Test Piece)

AnnotationAssertion(rdfs:isDefinedBy :TTO_0000055 <https://w3id.org/pmd/tto>)
AnnotationAssertion(rdfs:label :TTO_0000055 "Prüfkörper"@de)
AnnotationAssertion(rdfs:label :TTO_0000055 "Test Piece"@en)
AnnotationAssertion(rdfs:seeAlso :TTO_0000055 <https://w3id.org/pmd/co/2.0.8/TestPiece>)
AnnotationAssertion(<http://www.w3.org/2004/02/skos/core#definition> :TTO_0000055 "Part of a sample with specified dimensions, machined or un-machined, brought to a required condition for submission to a given test."@en)
AnnotationAssertion(<http://www.w3.org/2004/02/skos/core#definition> :TTO_0000055 "Teil einer Probe mit bestimmten Dimensionen, bearbeitet oder unbearbeitet, der in einen erforderlichen Zustand gebracht wird, um einer bestimmten Prüfung unterzogen zu werden."@de)
AnnotationAssertion(pmd:definitionSource :TTO_0000055 "EN 10021:2006-12 (European standardization committee: CEN/TC 459/SC 12/WG 4)")
SubClassOf(:TTO_0000055 ObjectIntersectionOf(<http://purl.obolibrary.org/obo/BFO_0000030> ObjectSomeValuesFrom(<http://purl.obolibrary.org/obo/BFO_0000196> pmd:PMD_0000975)))

# Class: :TTO_0000056 (End-Dicke)

AnnotationAssertion(rdfs:isDefinedBy :TTO_0000056 <https://w3id.org/pmd/ao/tto>)
AnnotationAssertion(rdfs:label :TTO_0000056 "End-Dicke"@de)
AnnotationAssertion(rdfs:label :TTO_0000056 "Thickness After Fracture"@en)
AnnotationAssertion(rdfs:seeAlso :TTO_0000056 <https://w3id.org/pmd/tto/ThicknessAfterFracture>)
AnnotationAssertion(<http://www.w3.org/2004/02/skos/core#definition> :TTO_0000056 "Diese Entität beschreibt die gemessene Dimension in einer Richtung eines Prüfstücks, wie sie vor der Prüfung gemessen wurde."@de)
AnnotationAssertion(<http://www.w3.org/2004/02/skos/core#definition> :TTO_0000056 "This entity describes the measured dimension in one direction of a test piece, as measured after the test."@en)
SubClassOf(:TTO_0000056 :TTO_0000006)

# Class: :TTO_0000057 (Umschaltpunkt)

AnnotationAssertion(rdfs:isDefinedBy :TTO_0000057 <https://w3id.org/pmd/ao/tto>)
AnnotationAssertion(rdfs:label :TTO_0000057 "Transition Point"@en)
AnnotationAssertion(rdfs:label :TTO_0000057 "Umschaltpunkt"@de)
AnnotationAssertion(rdfs:seeAlso :TTO_0000057 <https://w3id.org/pmd/tto/TransitionPoint>)
AnnotationAssertion(<http://www.w3.org/2004/02/skos/core#definition> :TTO_0000057 "Diese Entität beschreibt einen einzelnen Punkt, an dem ein Übergang von einer Bedingung oder einem Zustand in einen anderen erfolgt, z. B. der Punkt, an dem verschiedene Phasen von Materie im Gleichgewicht miteinander existieren können (auch Inversionspunkt genannt) oder wenn Prozessparameter geändert werden, die zu einem Übergang des Prozesses während seiner Ausführung führen."@de)
AnnotationAssertion(<http://www.w3.org/2004/02/skos/core#definition> :TTO_0000057 "This entity describes a single point at which a transition from one condition or state to another occurs, e.g. the point at which different phases of matter are capable of existing together in equilibrium (also called inversion point) or if process parameters are changed that will lead to a transition of the process during its execution."@en)
SubClassOf(:TTO_0000057 pmd:PMD_0000003)

# Class: :TTO_0000058 (Umschaltpunkt der Prüfgeschwindigkeit)

AnnotationAssertion(rdfs:isDefinedBy :TTO_0000058 <https://w3id.org/pmd/ao/tto>)
AnnotationAssertion(rdfs:label :TTO_0000058 "Transition Point Testing Rate"@en)
AnnotationAssertion(rdfs:label :TTO_0000058 "Umschaltpunkt der Prüfgeschwindigkeit"@de)
AnnotationAssertion(rdfs:seeAlso :TTO_0000058 <https://w3id.org/pmd/tto/TransitionPointTestingRate>)
AnnotationAssertion(<http://www.w3.org/2004/02/skos/core#definition> :TTO_0000058 "Diese Entität beschreibt den Umschaltpunkt der Prüfgeschwindigkeit während eines Analyse- / Testprozesses, z.B. den Punkt bezogen auf die Dehnung oder Spannung, an welchem die Prüfgeschwindigkeit während eines Zugversuchs geändert wird. Typischerweise ist dieser Punkt mit einer Abnahme des Extensometers (Dehnungsaufnehmers) vom Prüfkörper während eines dehnungsgeregelten Zugversuchs verbunden."@de)
AnnotationAssertion(<http://www.w3.org/2004/02/skos/core#definition> :TTO_0000058 "This entity describes the the transition point of the testing rate during an analysis / test process, e.g. the point referring to the strain or the stress at which the testing rate is changed during a tensile test. Typically, this transition point is associated with a removal of the extensometer from the test piece during a strain-controlled tensile test."@en)
SubClassOf(:TTO_0000058 :TTO_0000057)

# Class: :TTO_0000059 (Upper Yield Strength)

AnnotationAssertion(rdfs:isDefinedBy :TTO_0000059 <https://w3id.org/pmd/ao/tto>)
AnnotationAssertion(rdfs:label :TTO_0000059 "Obere Streckgrenze"@de)
AnnotationAssertion(rdfs:label :TTO_0000059 "Upper Yield Strength"@en)
AnnotationAssertion(rdfs:seeAlso :TTO_0000059 <https://w3id.org/pmd/tto/UpperYieldStrength>)
AnnotationAssertion(<http://www.w3.org/2004/02/skos/core#definition> :TTO_0000059 "höchste Spannung, bevor der erste Kraftabfall auftritt"@de)
AnnotationAssertion(<http://www.w3.org/2004/02/skos/core#definition> :TTO_0000059 "maximum value of stress prior to the first decrease in force"@en)
AnnotationAssertion(pmd:definitionSource :TTO_0000059 "DIN EN ISO 6892-1:2019"@en)
AnnotationAssertion(pmd:symbol :TTO_0000059 "R_eH"@en)
SubClassOf(:TTO_0000059 :TTO_0000009)

# Class: :TTO_0000060 (End-Breite)

AnnotationAssertion(rdfs:isDefinedBy :TTO_0000060 <https://w3id.org/pmd/ao/tto>)
AnnotationAssertion(rdfs:label :TTO_0000060 "End-Breite"@de)
AnnotationAssertion(rdfs:label :TTO_0000060 "Width After Fracture"@en)
AnnotationAssertion(rdfs:seeAlso :TTO_0000060 <https://w3id.org/pmd/tto/WidthAfterFracture>)
AnnotationAssertion(<http://www.w3.org/2004/02/skos/core#definition> :TTO_0000060 "Diese Entität beschreibt eine horizontale Messung eines Objekts (Prüfkörpers) im rechten Winkel zur Länge des Objekts (Prüfkörpers), wie sie nach einer Prüfung gemessen wird."@de)
AnnotationAssertion(<http://www.w3.org/2004/02/skos/core#definition> :TTO_0000060 "This entity describes a horizontal measurement of an object (test piece) taken at right angles to the length of the object (test piece), as measured after a test."@en)
SubClassOf(:TTO_0000060 :TTO_0000010)


)